Cleanups

theories/Dot/syn/pathrepl.v
@@ -73,8 +73,16 @@ Lemma path_wp_pure_swap p u :
   path_wp_pure p (λ w, w = u).
 Proof. split => Hp; exact: path_wp_pure_wand. Qed.
 
+(* XXX Unclear why is the substitution built-in. But beware of dropping that, as substitution and path replacement don't swap. *)
 Definition alias_paths_pure p q ρ :=
   path_wp_pure p.|[ρ] (λ vp, path_wp_pure q.|[ρ] (λ vq, vp = vq)).
+
+Lemma alias_path_pure_weaken p q ρ v:
+  alias_paths_pure p.|[ren (+1)] q.|[ren (+1)] (v .: ρ) ↔
+  alias_paths_pure p q ρ.
+Proof.
+  by rewrite /alias_paths_pure; f_equiv; rewrite hsubst_comp ren_scons.
+Qed.
 
 Lemma alias_paths_pure_refl_vl v ρ :
   alias_paths_pure (pv v) (pv v) ρ.
@@ -146,18 +154,95 @@ Section equivI_utils.
     P1 ≡ P2 ⊢@{PROP} (P1 ∧ Q) ≡ (P2 ∧ Q).
   Proof. apply (@f_equiv _ _ _ (λ P, P ∧ Q)%I). solve_proper. Qed.
 
-(*
-  Lemma and_equivI {PROP : sbi} (P1 P2 Q1 Q2 : PROP) :
-    P1 ≡ P2 ⊢@{PROP} Q1 ≡ Q2 -∗
-    (P1 ∧ Q1) ≡ (P2 ∧ Q2).
-  Proof.
-  Admitted. *)
-
   Lemma wand2_equivI {PROP : sbi} (P1 P2 Q : PROP) :
     P1 ≡ P2 ⊢@{PROP} (P1 -∗ Q) ≡ (P2 -∗ Q).
   Proof. apply (@f_equiv _ _ _ (λ P, P -∗ Q)%I). solve_proper. Qed.
 
 End equivI_utils.
+
+Ltac iProperness :=
+  repeat first
+  [ iEval (progress rewrite -(wp_equivI, exists_equivI, forall_equivI)); iIntros
+  (* f_equiv must come before those others for performance. *)
+  | iEval (progress rewrite -(f_equiv, and2_equivI, wand2_equivI, or2_equivI))
+  ].
+
+Section path_repl.
+  Context `{dlangG Σ}.
+  Implicit Types (φ: vl → iProp Σ).
+
+  Notation path_wp p φ := (@path_wp Σ p φ).
+  Notation path_wp_purel p Pv := (⌜path_wp_pure p Pv⌝%I : iProp Σ).
+
+  Lemma path_wp_pureable p Pv:
+    path_wp p (λ v, ⌜Pv v⌝) ⊣⊢ path_wp_purel p Pv.
+  Proof.
+    elim: p Pv => /= [//|p IHp l] Pv.
+    by rewrite -{}IHp; f_equiv => v; iIntros "!% /=".
+  Qed.
+
+  Global Instance path_wp_pureableI p Pv :
+    IntoPure (path_wp p (λ v, ⌜Pv v⌝))%I (path_wp_pure p Pv).
+  Proof. by rewrite /IntoPure path_wp_pureable. Qed.
+  Global Instance path_wp_pureableF p Pv :
+    FromPure false (path_wp p (λ v, ⌜Pv v⌝))%I (path_wp_pure p Pv).
+  Proof. by rewrite /FromPure/= path_wp_pureable. Qed.
+
+  Lemma path_wp_swap p u :
+    path_wp p (λ w, ⌜u = w⌝) ⊣⊢ path_wp p (λ w, ⌜w = u⌝).
+  Proof. iIntros "!%". by rewrite /= path_wp_pure_swap. Qed.
+
+  Definition alias_paths p q ρ : iProp Σ := ⌜alias_paths_pure p q ρ⌝.
+
+  Lemma alias_paths_refl_vl v ρ :
+    alias_paths (pv v) (pv v) ρ.
+  Proof. by iIntros "!%". Qed.
+
+  Lemma alias_paths_eq p q ρ:
+    alias_paths p q ρ ⊣⊢
+    ∃ v,
+      path_wp p.|[ρ] (λ vp : vl, ⌜vp = v⌝) ∧
+      path_wp q.|[ρ] (λ vq : vl, ⌜vq = v⌝).
+  Proof. iIntros "!%"; rewrite /= alias_paths_pure_eq. intuition. Qed.
+
+  Lemma simpl_alias_1 p vr ρ :
+    alias_paths p (pv vr) ρ ⊣⊢ path_wp_purel p.|[ρ] (λ w, w = vr.[ρ]).
+  Proof. done. Qed.
+
+  Lemma simpl_alias_2 p vr ρ :
+    alias_paths (pv vr) p ρ ⊣⊢ path_wp_purel p.|[ρ] (λ w, w = vr.[ρ]) .
+  Proof. by rewrite -path_wp_pure_swap. Qed.
+
+  (* Not provable through pure props for impure [φ]. *)
+  Lemma alias_paths_equiv p q ρ:
+    alias_paths_pure p q ρ ↔
+      (∃ u, path_wp_pure p.|[ρ] (λ vp, vp = u)) ∧
+      ∀ φ, path_wp p.|[ρ] φ ≡ path_wp q.|[ρ] φ.
+  Proof.
+    rewrite alias_paths_pure_eq; split.
+    - destruct 1 as (v & Hp & Hq).
+      split; first by [eauto]; intros φ.
+      rewrite !path_wp_eq. f_equiv => w.
+      rewrite !path_wp_pureable; do 2 f_equiv.
+      split => Hr; [ rewrite -(path_wp_pure_det Hp Hr)
+        | rewrite -(path_wp_pure_det Hq Hr)]; auto.
+    - destruct 1 as ((u & Hp) & Heq). exists u; split; first done.
+      (* Yes, completely insane. *)
+      apply (pure_soundness (M := iResUR Σ)).
+      iRevert (Hp). by rewrite -!path_wp_pureable Heq.
+  Qed.
+
+  Lemma alias_paths_equiv' p q ρ:
+    alias_paths p q ρ ⊣⊢
+      (∃ u, path_wp p.|[ρ] (λ vp, ⌜vp = u⌝)) ∧
+      ∀ φ, ⌜path_wp p.|[ρ] φ ≡ path_wp q.|[ρ] φ⌝.
+  Proof. iIntros "!%". apply alias_paths_equiv. Qed.
+
+  Lemma alias_paths_elim_eq φ p q ρ:
+    alias_paths_pure p q ρ →
+    path_wp p.|[ρ] φ ≡ path_wp q.|[ρ] φ.
+  Proof. intros ?%alias_paths_equiv. intuition. Qed.
+End path_repl.
 
 Definition psubst_path p q : path → path := fix F r :=
   match (decide (r = p)) with
@@ -175,18 +260,6 @@ Proof. elim: q => /= *; case_decide; by f_equal. Qed.
 
 Lemma psubst_path_self p q: p .p[ p := q ] = q.
 Proof. case: p => /= *; by rewrite decide_True. Qed.
-
-(* Useful ???*)
-Lemma psubst_path_eq p q r: psubst_path p q r =
-  match (decide (r = p)) with
-  | left _ => q
-  | _ =>
-    match r with
-    | pv _ => r
-    | pself r' l => pself (psubst_path p q r') l
-    end
-  end.
-Proof. by case: r. Qed.
 
 (* Alternative *)
 Reserved Notation "p1 ~pp[ p := q  ] p2" (at level 70).
@@ -240,127 +313,30 @@ where "T1 ~p[ p := q  ] T2" := (ty_path_repl p q T1 T2) .
 Lemma ty_path_repl_id p T1 T2 : T1 ~p[ p := p ] T2 → T1 = T2.
 Proof. intros Hr; dependent induction Hr; by rewrite // ?IHHr // psubst_path_id. Qed.
 
-Section path_repl.
+Section path_repl_2.
   Context `{dlangG Σ}.
   Implicit Types (φ: vl → iProp Σ).
 
-  Lemma path_wp_pureable p Pv:
-    path_wp p (λ v, ⌜Pv v⌝) ⊣⊢@{iPropI Σ} ⌜path_wp_pure p Pv⌝.
-  Proof.
-    elim: p Pv => /= [//|p IHp l] Pv.
-    by rewrite -{}IHp; f_equiv => v; iIntros "!% /=".
-  Qed.
+  Notation path_wp p φ := (@path_wp Σ p φ).
+  Notation path_wp_purel p Pv := (⌜path_wp_pure p Pv⌝%I : iProp Σ).
+  Notation alias_paths p q ρ := (@alias_paths Σ p q ρ).
 
-  Global Instance path_wp_pureableI p Pv :
-   IntoPure (@path_wp Σ p (λ v, ⌜Pv v⌝))%I (path_wp_pure p Pv).
-  Proof. by rewrite /IntoPure path_wp_pureable. Qed.
-  Global Instance path_wp_pureableF p Pv :
-   FromPure false  (@path_wp Σ p (λ v, ⌜Pv v⌝))%I (path_wp_pure p Pv).
-  Proof. by rewrite /FromPure/= path_wp_pureable. Qed.
+  (** Beware: we can do path replacement *before* substitution,
+      even tho substitution and path replacement don't commute nicely.
 
-  Lemma path_wp_swap p u :
-    path_wp p (λ w, ⌜u = w⌝) ⊣⊢@{iPropI Σ}
-    path_wp p (λ w, ⌜w = u⌝).
-  Proof. iIntros "!%". by rewrite /= path_wp_pure_swap. Qed.
+      As a special case, we get the less surprising:
+      [alias_paths_pure p r ids → path_wp q φ ≡ path_wp (q .p[p := r]) φ].
 
-  Definition alias_paths p q ρ : iProp Σ :=
-    path_wp p.|[ρ] (λ vp, path_wp q.|[ρ] (λ vq, ⌜vp = vq⌝))%I.
-
-  Lemma alias_paths_pureable p q ρ:
-    alias_paths p q ρ ⊣⊢ ⌜alias_paths_pure p q ρ⌝.
-  Proof.
-    rewrite /alias_paths/= -path_wp_pureable.
-    f_equiv => vp. apply path_wp_pureable.
-  Qed.
-
-  Global Instance alias_paths_pureableI p q ρ :
-   IntoPure (alias_paths p q ρ) (alias_paths_pure p q ρ).
-  Proof. by rewrite /IntoPure alias_paths_pureable. Qed.
-  Global Instance alias_paths_pureableF p q ρ :
-   FromPure false (alias_paths p q ρ) (alias_paths_pure p q ρ).
-  Proof. by rewrite /FromPure/= alias_paths_pureable. Qed.
-
-  Lemma alias_paths_refl_vl v ρ :
-    alias_paths (pv v) (pv v) ρ.
-  Proof. by iIntros "!%". Qed.
-
-  Lemma alias_paths_eq p q ρ:
-    alias_paths p q ρ ⊣⊢
-    ∃ v,
-      path_wp p.|[ρ] (λ vp : vl, ⌜vp = v⌝) ∧
-      path_wp q.|[ρ] (λ vq : vl, ⌜vq = v⌝).
-  Proof. iIntros "!%"; rewrite /= alias_paths_pure_eq. intuition. Qed.
-
-  Lemma alias_paths_symm p q ρ :
-    alias_paths p q ρ -∗ alias_paths q p ρ.
-  Proof.
-    rewrite !alias_paths_pureable; iIntros "!%".
-    exact: alias_paths_pure_symm.
-  Qed.
-
-  Lemma simpl_alias_1 p vr ρ :
-     alias_paths p (pv vr) ρ ⊣⊢ path_wp p.|[ρ] (λ w : vl, ⌜w = vr.[ρ]⌝) .
-  Proof. done. Qed.
-
-  Lemma simpl_alias_2 p vr ρ :
-     alias_paths (pv vr) p ρ ⊣⊢ path_wp p.|[ρ] (λ w : vl, ⌜w = vr.[ρ]⌝) .
-  Proof. exact: path_wp_swap. Qed.
-
-  Ltac iProperness :=
-    repeat first
-    [ iEval (progress rewrite -(wp_equivI, exists_equivI, forall_equivI)); iIntros
-    (* f_equiv must come before those others for performance. *)
-    | iEval (progress rewrite -(f_equiv, and2_equivI, wand2_equivI, or2_equivI))
-    ].
-
-  (* Not provable through pure props for impure [φ]. *)
-  Lemma alias_paths_equiv p q ρ:
-    alias_paths_pure p q ρ ↔
-      (∃ u, path_wp_pure p.|[ρ] (λ vp, vp = u)) ∧
-      ∀ φ, path_wp p.|[ρ] φ ≡ path_wp q.|[ρ] φ.
-  Proof.
-    rewrite alias_paths_pure_eq; split.
-    - destruct 1 as (v & Hp & Hq).
-      split; first by [eauto]; intros φ.
-      rewrite !path_wp_eq. f_equiv => w.
-      rewrite !path_wp_pureable; do 2 f_equiv.
-      split => Hr; [ rewrite -(path_wp_pure_det Hp Hr)
-        | rewrite -(path_wp_pure_det Hq Hr)]; auto.
-    - destruct 1 as ((u & Hp) & Heq). exists u; split; first done.
-      (* Yes, completely insane. *)
-      apply (pure_soundness (M := iResUR Σ)).
-      iRevert (Hp). by rewrite -!path_wp_pureable Heq.
-  Qed.
-
-  Lemma alias_paths_equiv' p q ρ:
-    ⌜alias_paths_pure p q ρ⌝ ⊣⊢@{iPropI Σ}
-      (∃ u, path_wp p.|[ρ] (λ vp, ⌜vp = u⌝)) ∧
-      ∀ φ, ⌜path_wp p.|[ρ] φ ≡ path_wp q.|[ρ] φ⌝.
-  Proof. iIntros "!%". apply alias_paths_equiv. Qed.
-
-  Lemma alias_paths_elim_eq φ p q ρ:
-    alias_paths_pure p q ρ →
-    path_wp p.|[ρ] φ ≡ path_wp q.|[ρ] φ.
-  Proof. intros ?%alias_paths_equiv. intuition. Qed.
-
-  Lemma alias_paths_elim_eq' φ p q ρ:
-    ⌜alias_paths_pure p q ρ⌝ ⊢@{iPropI Σ}
-    ⌜path_wp p.|[ρ] φ ≡ path_wp q.|[ρ] φ⌝.
-  Proof. iIntros "!%". apply alias_paths_elim_eq. Qed.
-
-  Lemma alias_paths_elim_wand p q ρ φ:
-    ⌜alias_paths_pure p q ρ⌝ ⊢@{iPropI Σ}
-    path_wp p.|[ρ] φ -∗ path_wp q.|[ρ] φ.
-  Proof. rewrite (alias_paths_elim_eq' φ). iIntros (->) "$". Qed.
-
-  Lemma path_replacement_equiv_plain {p r ρ} q (φ : vl → iProp Σ):
+      But we do need the general form. *)
+  Lemma path_replacement_equiv {p r ρ} q (φ : vl → iProp Σ):
     alias_paths_pure p r ρ →
     path_wp q.|[ρ] φ ≡ path_wp (q .p[p := r]).|[ρ] φ.
   Proof.
-    elim: q φ => [w | q IHq l] φ /=; case_decide; simplify_eq/=.
-    - apply (alias_paths_elim_eq φ (pv w) r).
+    elim: q φ => [w | q IHq l] φ /=; case_decide.
+    - simplify_eq. apply (alias_paths_elim_eq φ (pv w) r).
     - done.
-    - rewrite /= !path_wp_eq alias_paths_pure_eq /=.
+    - simplify_eq.
+      rewrite /= !path_wp_eq alias_paths_pure_eq /=.
       destruct 1 as (vr & (vq & Hq & w & Hl & ->)%path_wp_pure_eq & Hr).
       iSplit.
       + iDestruct 1 as (vq' Hq' vr' Hl') "Hφ".
@@ -372,101 +348,37 @@ Section path_repl.
     - exact: IHq.
   Qed.
 
-  Lemma path_replacement_equiv_plain' {p r ρ} q (φ : vl → iProp Σ):
-    ⌜alias_paths_pure p r ρ⌝ ⊢@{iPropI Σ}
-    path_wp q.|[ρ] φ ≡ path_wp (q .p[p := r]).|[ρ] φ.
-  Proof. iIntros (?) "!%". exact: path_replacement_equiv_plain. Qed.
-
-  (* Lemma path_replacement_equiv_pure {p r ρ} q (φ : vl → iProp Σ):
-    alias_paths p r ρ ⊢@{iPropI Σ}
-    (⌜ path_wp q.|[ρ] φ ≡ path_wp (q .p[p := r]).|[ρ] φ⌝)%I.
+  Lemma path_replacement_equiv_alt {p r ρ} q q' (φ : vl → iProp Σ):
+    q ~pp[ p := r ] q' →
+    alias_paths_pure p r ρ →
+    path_wp q.|[ρ] φ ≡ path_wp q'.|[ρ] φ.
   Proof.
-    elim: q φ => [w | q IHq l] φ /=;
-     case_decide; simplify_eq/=.
-    (* - apply (alias_paths_elim_eq φ (pv w) r).
-    - by iIntros.
-    - rewrite /= !path_wp_eq alias_paths_eq /=.
-      iDestruct 1 as (vr) "[Hq' #Hr]".
-      iDestruct (path_wp_eq with "Hq'") as (vq) "#[Hq A]";
-        iDestruct "A" as %(? & Hl & ->).
-      iApply prop_ext; iModIntro; iSplit.
-      + iDestruct 1 as (vq') "[Hq' A]"; iDestruct "A" as (vr' Hl') "Hφ".
-        iDestruct (path_wp_det with "Hq Hq'") as %<-; iClear "Hq Hq'".
-        by objLookupDet; eauto.
-      + iDestruct 1 as (vr') "[Hr' Hφ]".
-        iDestruct (path_wp_det with "Hr Hr'") as %<-; iClear "Hr'".
-        eauto.
-    - iIntros. by iApply IHq.
-  Qed. *)
-  Admitted.
-
-  Lemma path_replacement_equiv_plain2 {p r ρ} q (φ : vl → iProp Σ):
-    alias_paths p r ρ ⊢@{iPropI Σ}
-    path_wp q.|[ρ] φ ≡ path_wp (q .p[p := r]).|[ρ] φ.
-  Proof. rewrite path_replacement_equiv_pure. by iIntros (<-). Qed. *)
-
-  Lemma rewrite_tsel_psubst2 p q l ρ v r:
-    ⌜alias_paths_pure p r ρ⌝ ⊢@{iPropI Σ}
-    ⟦ TSel q l ⟧ ρ v ≡ ⟦ TSel (q .p[ p := r ]) l ⟧ ρ v.
-  Proof. exact: path_replacement_equiv_plain'. Qed.
-
-  (* That's false. *)
-  (* Lemma path_replacement_equiv_0 {p r ρ} q:
-    alias_paths p r ρ ⊢@{iPropI Σ}
-    alias_paths q (q .p[p := r]) ρ.
-  Proof.
-    elim: q => [w | q IHq l] /=; case_decide; simplify_eq/=.
-    - by iIntros.
-    - rewrite -alias_paths_refl_vl. by iIntros.
-    - by iIntros.
-    - rewrite /= IHq !alias_paths_eq /=.
-      iDestruct 1 as (vr) "#[Hq Hqr]".
-      (* We don't know that [pself q l] terminates! *)
-  Abort. *)
-
-  Lemma path_replacement_equiv p q r ρ (φ : vl → iProp Σ):
-    ⌜alias_paths_pure p r ρ⌝ ⊢@{iPropI Σ}
-    □(path_wp q.|[ρ] φ ∗-∗ path_wp (q .p[p := r]).|[ρ] φ).
-  Proof.
-    iIntros "#H !>".
-    iRewrite -(path_replacement_equiv_plain' q φ with "H").
-    by rewrite -wand_iff_refl.
+    move => Hrepl.
+    elim: Hrepl φ => [| p1 p2 l Hrepl IHrepl] φ /=.
+    exact: alias_paths_elim_eq.
+    apply IHrepl.
   Qed.
 
-  Lemma alias_path_pure_weaken p q ρ v:
-     alias_paths_pure p.|[ren (+1)] q.|[ren (+1)] (v .: ρ) ↔
-     alias_paths_pure p q ρ.
-  Proof.
-    by rewrite /alias_paths_pure; f_equiv; rewrite hsubst_comp ren_scons.
-  Qed.
+  Lemma path_replacement_equiv' {p r ρ} q (φ : vl → iProp Σ):
+    alias_paths p r ρ ⊢
+    path_wp q.|[ρ] φ ≡ path_wp (q .p[p := r]).|[ρ] φ.
+  Proof. iIntros (?) "!%". exact: path_replacement_equiv. Qed.
 
-  Lemma rewrite_ty_path_repl_plain p q T1 T2 ρ v:
+  Lemma rewrite_ty_path_repl p q T1 T2 ρ v:
     T1 ~p[ p := q ] T2 →
     alias_paths_pure p q ρ →
     ⟦ T1 ⟧ ρ v ≡ ⟦ T2 ⟧ ρ v.
   Proof.
     move => Hrew; move: v ρ.
     induction Hrew => v ρ He /=; properness;
-      by [|exact: path_replacement_equiv_plain|iApply IHHrew; rewrite ?alias_path_pure_weaken].
+      by [|exact: path_replacement_equiv|iApply IHHrew; rewrite ?alias_path_pure_weaken].
   Qed.
 
-  Lemma rewrite_ty_path_repl_plain' p q T1 T2 ρ v:
+  Lemma rewrite_ty_path_repl' p q T1 T2 ρ v:
     T1 ~p[ p := q ] T2 →
-    alias_paths p q ρ ⊢@{iPropI Σ} (* p : q.type *)
+    alias_paths p q ρ ⊢ (* p : q.type *)
     ⟦ T1 ⟧ ρ v ≡ ⟦ T2 ⟧ ρ v.
-  Proof. iIntros "!% /=". exact: rewrite_ty_path_repl_plain. Qed.
-
-  (* Lemma rewrite_ty_path_repl_plain'_slow p q T1 T2 ρ v:
-    T1 ~p[ p := q ] T2 →
-    ⌜alias_paths_pure p q ρ⌝ ⊢@{iPropI Σ} (* p : q.type *)
-    ⟦ T1 ⟧ ρ v ≡ ⟦ T2 ⟧ ρ v.
-  Proof.
-    move => Hrew; move: v ρ.
-    induction Hrew => v ρ;
-      iIntros "/= #H"; iProperness; last
-      iApply path_replacement_equiv_plain';
-      try by [|iApply IHHrew; rewrite ?alias_path_pure_weaken].
-  Qed. *)
+  Proof. iIntros "!%". exact: rewrite_ty_path_repl. Qed.
 
   (* Lemma TMu_E Γ T v: Γ ⊨ tv v : TMu T -∗ Γ ⊨ tv v : T.|[ids 0/] .p [.
   Proof. by rewrite TMu_equiv. Qed.
@@ -474,98 +386,4 @@ Section path_repl.
   Lemma TMu_I Γ T v: Γ ⊨ tv v : T.|[v/] -∗ Γ ⊨ tv v : TMu T.
   Proof. by rewrite TMu_equiv. Qed. *)
 
-
-      (* rewrite -?exists_equivI; iIntros; rewrite -?f_equiv.
-    1-2: rewrite -forall_equivI; iIntros (w).
-    by iRewrite (IHHrew w with "H").
-    rewrite -f_equiv -wp_equivI; iIntros.
-    1-2: by iApply IHHrew; rewrite // hsubst_comp subst_comp ren_scons.
-    all: rewrite -exists_equivI; iIntros (w); rewrite -!f_equiv.
-    by iRewrite (IHHrew w with "H").
-    rewrite -?and2_equivI.
-    rewrite -f_equiv.
-    all: rewrite -forall_equivI; iIntros (v0); by iRewrite (IHHrew v0 with "H").
-  Qed. *)
-      (* rewrite -f_equiv -wp_equivI; iIntros.
-
-       iApply "H".
-    (* iDestruct 1 as (t Heq) "#H1"; iExists t; iSplit; first done; iIntros "!>!>" (w) "#Ha"; *)
-      by iRewrite (IHHrew w with "H").
-      iApply internal_eq_proper. exist_proper.
-    f_equiv.
-    properness.
-    iDestruct 1 as "H1".
-    iDestruct 1 as (t Heq) "H1". iExists t; iSplit; first done; iIntros "!>!>" (w) "#Ha"; iApply "H1"; by iApply IHHrew. *)
-
-    (* move HE: (pv vr) => q Hrew.
-    iInduction Hrew as [] "IHHrew" forall (v ρ vr HE); subst q;
-      last iApply rewrite_tsel_psubst2; iIntros "/= #H";
-      try by iRewrite ("IHHrew" $! v with "[//] H").
-      try by iRewrite ("IHHrew" with "[//] H").
-       iApply prop_ext; iModIntro; iSplit. *)
-
-(* Axiom skip: forall a, a. *)
-  (* Special cases, any use? *)
-  (* Lemma path_replacement_equiv_plain_special {p vr ρ} q (φ : vl → iProp Σ):
-    path_wp p.|[ρ] (λ w, ⌜ w = vr.[ρ] ⌝) ⊢@{iPropI Σ}
-    path_wp q.|[ρ] φ ≡ path_wp (q .p[p := pv vr]).|[ρ] φ.
-  Proof. rewrite -path_replacement_equiv_plain' -simpl_alias_1.
-  by iIntros "!%". Qed.
-
-  Lemma rewrite_tsel_psubst2_special p q l ρ v vr:
-    path_wp p.|[ρ] (λ w, ⌜ w = vr.[ρ] ⌝) ⊢@{iPropI Σ}
-    ⟦ TSel q l ⟧ ρ v ≡ ⟦ TSel (q .p[ p := pv vr ]) l ⟧ ρ v.
-  Proof. exact: path_replacement_equiv_plain_special. Qed. *)
-
-  (* Lemma rewrite_ty_path_repl p T1 T2 ρ v vr:
-    T1 ~p[ p := pv vr ] T2 →
-    path_wp p.|[ρ] (λ w, ⌜ w = vr.[ρ] ⌝) ⊢@{iPropI Σ}
-    □(⟦ T1 ⟧ ρ v ∗-∗ ⟦ T2 ⟧ ρ v).
-  Proof.
-    (* V1: gets type error at Qed, due to [dependent induction]. *)
-    intros Hrew; move: v ρ; dependent induction Hrew => v ρ;
-    (* V2 *)
-    (* move HE: (pv vr) => q; move => Hrew; move: v ρ vr HE. induction Hrew => v ρ vr HE; subst q; *)
-      last apply skip; iIntros "/= #H !>"; iSplit.
-    1-4: iIntros "[??]"; iFrame; by iApply IHHrew.
-    1-4: iIntros "[?|?]"; iFrame; by (iLeft + iRight); iApply IHHrew.
-    1-2: iIntros "? !>"; by iApply IHHrew.
-    1-2: iDestruct 1 as (t Heq) "#H1"; iExists t; iSplit; first done; iIntros "!>!>" (w) "#Ha"; iApply "H1"; by iApply IHHrew.
-    1-2: iDestruct 1 as (t Heq) "#H1"; iExists t; iSplit; first done; iIntros "!>!>" (w) "#Ha";
-      iApply (wp_wand with "(H1 Ha)").
-    1-4: iIntros; iApply IHHrew; rewrite // hsubst_comp subst_comp ren_scons; iApply "H".
-    1-2: iDestruct 1 as (d Hl vm Heq) "H1"; iExists d; iSplit; first done; iExists vm; iSplit; first done; by iApply IHHrew.
-    1-4: iDestruct 1 as (d Hl ψ) "[Hl #[HL HU]]"; iExists d; iSplit; first done; iExists ψ; iSplit; first done; iModIntro; iSplit; iIntros.
-      1-8: try ((iApply "HL" || iApply "HU"); by [iApply IHHrew|]).
-      1-2: iApply IHHrew; by [iApply "HL"|iApply "HU"|].
-  Qed. *)
-
-  (* Looks very false. *)
-  (* Lemma swap_substs p q r ρ: (q .p[ p := r ]).|[ren ρ] = q.|[ren ρ] .p[ p.|[ren ρ] := r.|[ren ρ]].
-  Proof.
-    induction q eqn:Heq; cbn; case_decide; try by simplify_eq/=; rewrite 1?decide_True.
-    case_decide => //=.
-    rewrite H1. f_equal.
-    simplify_eq/=.
-  elim: q => /= [v | q IHq l]; case_decide; simplify_eq/=; try by rewrite 1?decide_True.
-
-  rewrite decide_False; simplify_eq/=. done. naive_solver. congruence. *)
-
-  (* Lemma path_replacement p q vr ρ φ:
-    □path_wp p.|[ρ] (λ w, ⌜ w = vr.[ρ] ⌝) ⊢@{iPropI Σ}
-    □(path_wp q.|[ρ] φ -∗ path_wp (q .p[p := pv vr]).|[ρ] φ).
-  Proof.
-    iIntros "#Heq !> HA".
-    (* rewrite (path_replacement_equiv_plain q φ); by iApply (internal_eq_iff with "Heq"). *)
-    iApply (path_replacement_equiv with "Heq HA").
-  Qed.
-
-  Lemma path_replacement_2 p q vr ρ φ:
-    □path_wp p.|[ρ] (λ w, ⌜ w = vr.[ρ] ⌝) ⊢@{iPropI Σ}
-    □(path_wp (q .p[p := pv vr]).|[ρ] φ -∗ path_wp q.|[ρ] φ).
-  Proof.
-    iIntros "#Heq !> HA".
-    iApply (path_replacement_equiv with "Heq HA").
-  Qed. *)
-
-End path_repl.
+End path_repl_2.
