theories/Dot/misc/path_repl_dead.v
@@ -1,0 +1,167 @@
+From iris.proofmode Require Import tactics.
+
+From D.Dot.lr Require Import unary_lr.
+From D.Dot.syn Require Import syn pathrepl.
+
+Implicit Types
+         (T : ty) (v w : vl) (t : tm) (d : dm) (ds : dms) (p q : path)
+         (Γ : ctx) (vs : vls) (l : label).
+
+Implicit Types (Pv : vl → Prop).
+Set Nested Proofs Allowed.
+
+(* Useful ???*)
+Lemma psubst_path_eq p q r: psubst_path p q r =
+  match (decide (r = p)) with
+  | left _ => q
+  | _ =>
+    match r with
+    | pv _ => r
+    | pself r' l => pself (psubst_path p q r') l
+    end
+  end.
+Proof. by case: r. Qed.
+
+Definition path_wp_purel {Σ} p Pv : iProp Σ := (⌜path_wp_pure p Pv⌝%I : iProp Σ).
+Global Arguments path_wp_purel /.
+
+Section path_repl.
+  Context `{dlangG Σ}.
+  Implicit Types (φ: vl → iProp Σ).
+
+  Notation alias_paths p q ρ := (@alias_paths Σ p q ρ).
+(*
+  Lemma and_equivI {PROP : sbi} (P1 P2 Q1 Q2 : PROP) :
+    P1 ≡ P2 ⊢@{PROP} Q1 ≡ Q2 -∗
+    (P1 ∧ Q1) ≡ (P2 ∧ Q2).
+  Proof.
+  Admitted. *)
+
+  (* Notation path_wp_purel p Pv := (@path_wp_purel Σ p Pv). *)
+  Lemma alias_paths_symm p q ρ :
+    alias_paths p q ρ -∗ alias_paths q p ρ.
+  Proof. iIntros "!%". exact: alias_paths_pure_symm. Qed.
+
+  Lemma alias_paths_elim_eq' φ p q ρ:
+    alias_paths p q ρ ⊢
+    ⌜path_wp p.|[ρ] φ ≡ path_wp q.|[ρ] φ⌝.
+  Proof. iIntros "!%". apply alias_paths_elim_eq. Qed.
+
+  Lemma alias_paths_elim_wand φ p q ρ:
+    alias_paths_pure p q ρ →
+    path_wp p.|[ρ] φ ⊢ path_wp q.|[ρ] φ.
+  Proof. iIntros (->%(alias_paths_elim_eq φ)) "$". Qed.
+  Lemma alias_paths_elim_wand' φ p q ρ:
+    alias_paths p q ρ ⊢
+    path_wp p.|[ρ] φ -∗ path_wp q.|[ρ] φ.
+  Proof. iIntros (->%(alias_paths_elim_wand φ)) "$". Qed.
+
+
+  Lemma rewrite_tsel_psubst2 p q l ρ v r:
+    alias_paths p r ρ ⊢
+    ⟦ TSel q l ⟧ ρ v ≡ ⟦ TSel (q .p[ p := r ]) l ⟧ ρ v.
+  Proof. exact: path_replacement_equiv'. Qed.
+
+  (* That's false, as we don't know that q terminates from the hyp. *)
+  (* Lemma path_replacement_equiv_0 {p r ρ} q:
+    alias_paths p r ρ ⊢@{iPropI Σ}
+    alias_paths q (q .p[p := r]) ρ.
+  Proof.
+    elim: q => [w | q IHq l] /=; case_decide; simplify_eq/=.
+    - by iIntros.
+    - rewrite -alias_paths_refl_vl. by iIntros.
+    - by iIntros.
+    - rewrite /= IHq !alias_paths_eq /=.
+      iDestruct 1 as (vr) "#[Hq Hqr]".
+      (* We don't know that [pself q l] terminates! *)
+  Abort. *)
+
+  (* Lemma rewrite_ty_path_repl'_slow p q T1 T2 ρ v:
+    T1 ~p[ p := q ] T2 →
+    ⌜alias_paths_pure p q ρ⌝ ⊢@{iPropI Σ} (* p : q.type *)
+    ⟦ T1 ⟧ ρ v ≡ ⟦ T2 ⟧ ρ v.
+  Proof.
+    move => Hrew; move: v ρ.
+    induction Hrew => v ρ;
+      iIntros "/= #H"; iProperness; last
+      iApply path_replacement_equiv';
+      try by [|iApply IHHrew; rewrite ?alias_path_pure_weaken].
+  Qed. *)
+
+
+      (* rewrite -?exists_equivI; iIntros; rewrite -?f_equiv.
+    1-2: rewrite -forall_equivI; iIntros (w).
+    by iRewrite (IHHrew w with "H").
+    rewrite -f_equiv -wp_equivI; iIntros.
+    1-2: by iApply IHHrew; rewrite // hsubst_comp subst_comp ren_scons.
+    all: rewrite -exists_equivI; iIntros (w); rewrite -!f_equiv.
+    by iRewrite (IHHrew w with "H").
+    rewrite -?and2_equivI.
+    rewrite -f_equiv.
+    all: rewrite -forall_equivI; iIntros (v0); by iRewrite (IHHrew v0 with "H").
+  Qed. *)
+      (* rewrite -f_equiv -wp_equivI; iIntros.
+
+       iApply "H".
+    (* iDestruct 1 as (t Heq) "#H1"; iExists t; iSplit; first done; iIntros "!>!>" (w) "#Ha"; *)
+      by iRewrite (IHHrew w with "H").
+      iApply internal_eq_proper. exist_proper.
+    f_equiv.
+    properness.
+    iDestruct 1 as "H1".
+    iDestruct 1 as (t Heq) "H1". iExists t; iSplit; first done; iIntros "!>!>" (w) "#Ha"; iApply "H1"; by iApply IHHrew. *)
+
+    (* move HE: (pv vr) => q Hrew.
+    iInduction Hrew as [] "IHHrew" forall (v ρ vr HE); subst q;
+      last iApply rewrite_tsel_psubst2; iIntros "/= #H";
+      try by iRewrite ("IHHrew" $! v with "[//] H").
+      try by iRewrite ("IHHrew" with "[//] H").
+       iApply prop_ext; iModIntro; iSplit. *)
+
+(* Axiom skip: forall a, a. *)
+  (* Special cases, any use? *)
+  (* Lemma path_replacement_equiv_special {p vr ρ} q (φ : vl → iProp Σ):
+    path_wp p.|[ρ] (λ w, ⌜ w = vr.[ρ] ⌝) ⊢@{iPropI Σ}
+    path_wp q.|[ρ] φ ≡ path_wp (q .p[p := pv vr]).|[ρ] φ.
+  Proof. rewrite -path_replacement_equiv' -simpl_alias_1.
+  by iIntros "!%". Qed.
+
+  Lemma rewrite_tsel_psubst2_special p q l ρ v vr:
+    path_wp p.|[ρ] (λ w, ⌜ w = vr.[ρ] ⌝) ⊢@{iPropI Σ}
+    ⟦ TSel q l ⟧ ρ v ≡ ⟦ TSel (q .p[ p := pv vr ]) l ⟧ ρ v.
+  Proof. exact: path_replacement_equiv_special. Qed. *)
+
+  (* Lemma rewrite_ty_path_repl p T1 T2 ρ v vr:
+    T1 ~p[ p := pv vr ] T2 →
+    path_wp p.|[ρ] (λ w, ⌜ w = vr.[ρ] ⌝) ⊢@{iPropI Σ}
+    □(⟦ T1 ⟧ ρ v ∗-∗ ⟦ T2 ⟧ ρ v).
+  Proof.
+    (* V1: gets type error at Qed, due to [dependent induction]. *)
+    intros Hrew; move: v ρ; dependent induction Hrew => v ρ;
+    (* V2 *)
+    (* move HE: (pv vr) => q; move => Hrew; move: v ρ vr HE. induction Hrew => v ρ vr HE; subst q; *)
+      last apply skip; iIntros "/= #H !>"; iSplit.
+    1-4: iIntros "[??]"; iFrame; by iApply IHHrew.
+    1-4: iIntros "[?|?]"; iFrame; by (iLeft + iRight); iApply IHHrew.
+    1-2: iIntros "? !>"; by iApply IHHrew.
+    1-2: iDestruct 1 as (t Heq) "#H1"; iExists t; iSplit; first done; iIntros "!>!>" (w) "#Ha"; iApply "H1"; by iApply IHHrew.
+    1-2: iDestruct 1 as (t Heq) "#H1"; iExists t; iSplit; first done; iIntros "!>!>" (w) "#Ha";
+      iApply (wp_wand with "(H1 Ha)").
+    1-4: iIntros; iApply IHHrew; rewrite // hsubst_comp subst_comp ren_scons; iApply "H".
+    1-2: iDestruct 1 as (d Hl vm Heq) "H1"; iExists d; iSplit; first done; iExists vm; iSplit; first done; by iApply IHHrew.
+    1-4: iDestruct 1 as (d Hl ψ) "[Hl #[HL HU]]"; iExists d; iSplit; first done; iExists ψ; iSplit; first done; iModIntro; iSplit; iIntros.
+      1-8: try ((iApply "HL" || iApply "HU"); by [iApply IHHrew|]).
+      1-2: iApply IHHrew; by [iApply "HL"|iApply "HU"|].
+  Qed. *)
+
+  (* Looks very false. *)
+  (* Lemma swap_substs p q r ρ: (q .p[ p := r ]).|[ren ρ] = q.|[ren ρ] .p[ p.|[ren ρ] := r.|[ren ρ]].
+  Proof.
+    induction q eqn:Heq; cbn; case_decide; try by simplify_eq/=; rewrite 1?decide_True.
+    case_decide => //=.
+    rewrite H1. f_equal.
+    simplify_eq/=.
+  elim: q => /= [v | q IHq l]; case_decide; simplify_eq/=; try by rewrite 1?decide_True.
+
+  rewrite decide_False; simplify_eq/=. done. naive_solver. congruence. *)
+End path_repl.
